
$$\begin{aligned}A+B&=B+A&(\text{commutative law})\\c\left(A+B\right)&=cA+cB&(\text{distributive law})\\A+\left(B+C\right)&=(A+B)+C&(\text{associative law}).\end{aligned}$$

$$\begin{aligned}&AB\neq BA&&(\text{the commutative “law” is }usually\textit{ broken})\\&A\left(B+C\right)=AB+AC&&(\text{distributive law from the left})\\&(A+B)C=AC+BC&&(\text{distributive law from the right})\\&A\left(BC\right)=(AB)C&&(\text{associative law for }ABC)(\textit{parentheses not needed}).\end{aligned}$$

- 列 * 行 ---> 矩阵

$$\begin{bmatrix}
 \\\  
 \\

\end{bmatrix}
\begin{bmatrix}
  &  &
\end{bmatrix}
\Rightarrow \begin{bmatrix}
  &  & \\
  &  & \\
  &  &
\end{bmatrix}$$
- 行 * 列 ---> 数
$$
\begin{bmatrix}
  &  &
\end{bmatrix}
\begin{bmatrix}
 \\\  
 \\
\end{bmatrix}
\Rightarrow
number$$
- 左侧行操作
  $$
  \begin{bmatrix}
  &  &
\end{bmatrix}A
\Rightarrow
combination \ of \ the \ rows \ of \ A
  $$
- 右侧列操作
 $$
 A\begin{bmatrix}
 \\\  
 \\
\end{bmatrix}
\Rightarrow
combination \ of \ the \ columns\ of \ A
$$